@prefix dpp: <https://example.org/DPP_ontology#> .
@prefix owl: <http://www.w3.org/2002/07/owl#> .
@prefix rdfs: <http://www.w3.org/2000/01/rdf-schema#> .
@prefix xsd: <http://www.w3.org/2001/XMLSchema#> .

<https://example.org/DPP_ontology> a owl:Ontology .

dpp:ConformityCertificates a owl:Class ;
    rdfs:label "Conformity Certificates"@en ;
    rdfs:comment "The conformity certificates for a product."@en ;
    rdfs:subClassOf dpp:Certification .

dpp:EnergyEfficiencyRating a owl:Class ;
    rdfs:label "Energy Efficiency Rating"@en ;
    rdfs:comment "The energy efficiency rating of a product, e.g., ENERGY STAR and DesignLights Consortium (DLC) for lighting products."@en ;
    rdfs:subClassOf dpp:Certification .

dpp:EnvironmentalCertification a owl:Class ;
    rdfs:label "Environmental Certification"@en ;
    rdfs:comment "The environmental certifications of a product, e.g., RoHS, REACH (https://www.assent.com/blog/difference-reach-rohs-compliance/)."@en ;
    rdfs:subClassOf dpp:Certification .

dpp:RegulatoryCompliance a owl:Class ;
    rdfs:label "Regulatory Compliance"@en ;
    rdfs:comment "Indicates whether a product complies with applicable building codes and regulations."@en ;
    rdfs:subClassOf dpp:Certification .

dpp:SafetyCertification a owl:Class ;
    rdfs:label "Safety Certification"@en ;
    rdfs:comment "The safety certifications of a product, e.g., UL, CE."@en ;
    rdfs:subClassOf dpp:Certification .

dpp:certificationAuthority a owl:DatatypeProperty ;
    rdfs:label "Certification Authority "@en ;
    rdfs:comment "The organization or body that issued the certification"@en ;
    rdfs:domain dpp:Certification ;
    rdfs:range xsd:string .

dpp:certificationIdentifier a owl:DatatypeProperty ;
    rdfs:label "Certification Identifier"@en ;
    rdfs:comment "A unique identifier for the certification, such as a certificate number"@en ;
    rdfs:domain dpp:Certification ;
    rdfs:range xsd:string .

dpp:certificationName a owl:DatatypeProperty ;
    rdfs:label "Certification Name"@en ;
    rdfs:comment "The name of the certification"@en ;
    rdfs:domain dpp:Certification ;
    rdfs:range xsd:string .

dpp:certificationScope a owl:DatatypeProperty ;
    rdfs:label "Certification Scope"@en ;
    rdfs:comment "A description of the scope of the certification, i.e., the aspects or activities it covers."@en ;
    rdfs:domain dpp:Certification ;
    rdfs:range xsd:string .

dpp:certificationStatus a owl:DatatypeProperty ;
    rdfs:label "Certification Status"@en ;
    rdfs:comment "The current status of the certification, e.g., active, expired, revoked."@en ;
    rdfs:domain dpp:Certification ;
    rdfs:range xsd:string .

dpp:expiryDate a owl:DatatypeProperty ;
    rdfs:label "Expiry Date"@en ;
    rdfs:comment "The date when the certification expires, if applicable."@en ;
    rdfs:domain dpp:Certification ;
    rdfs:range xsd:date .

dpp:hasCertification a owl:ObjectProperty ;
    rdfs:label "has certification"@en ;
    rdfs:comment "Links the product to its Certification"@en ;
    rdfs:domain dpp:Product ;
    rdfs:range dpp:Certification .

dpp:issueDate a owl:DatatypeProperty ;
    rdfs:label "Issue Date"@en ;
    rdfs:comment "The date when the certification was issued."@en ;
    rdfs:domain dpp:Certification ;
    rdfs:range xsd:date .

dpp:Certification a owl:Class ;
    rdfs:label "Product Certification"@en ;
    rdfs:comment "A formal recognition or validation of a product or Manufacturer's compliance with specific standards, regulations, or guidelines."@en .

